\documentclass{article}
  \usepackage{amsmath}
  \usepackage{amssymb}
  \usepackage{amsthm}
  \newtheorem{theorem}{Theorem}[section]
  \newcommand{\setcomp}[1] {{#1}^{\mathsf{c}}}

\begin{document}

\title{Prove for theorems of axiomatic boolean algebra}

\begin{theorem}[Idempotent laws]
\label{idempotent}
\[ x + x = x \]
\[ x * x = x \]
\end{theorem}

\begin{proof}
\begin{align*}
x + x & = (x + x) * 1 \\
      & = (x + x) * (x + x') \longleftarrow \text{distributive laws} \\
      & = x + (x * x') \\
      & = x + 0 \\
      & = x
\end{align*}
\end{proof}

\begin{proof}
\begin{align*}
x * x & = (x * x) + 0 \\
      & = (x * x) + (x * x') \longleftarrow \text{distributive laws} \\
      & = x * (x + x') \\
      & = x * 1 \\
      & = x
\end{align*}
\end{proof}

Absorption Laws:
\begin{equation}
x + (x * y) = x
\end{equation}

\begin{equation}
x * (x + y) = x
\end{equation}

\begin{proof}
\begin{align*}
x + (x * y) & = (x * 1) + (x * y)  \longleftarrow \text{distributive laws} \\
            & = x * (1 + y) \\
            & = x * 1 \\
            & = x
\end{align*}
\end{proof}

\begin{proof}
\begin{align*}
x * (x + y) & = x * x + x * y \longleftarrow \text{distributive laws} \\
            & = x + (x * y) \\
            & = x
\end{align*}
\end{proof}

Associative Laws:
\begin{equation}
x + (y + z) = (x + y) + z
\end{equation}
\begin{equation}
(x * y) * z = x * (y * z)
\end{equation}

\begin{proof}
let $A = [x + (y + z)] * [(x + y) + z]$, then:
\begin{align*}
A & = [(x + y) + z] * [x + (y + z)] \\
  & = [(x + y) + z] * x + [(x + y) + z] * (y + z) \\
  & = [(x + y) * x + x * z] + \{[(x + y) + z] * y + [(x + y) + z] * z\} \\
  & = [x + x * z] + \{[(x + y) * y + z * y] + z\} \\
  & = x + \{(y + z * y) + z\} \\
  & = x + (y + z)
\end{align*}
but also:

\begin{align*}
A & = [x + (y + z)] * [(x + y) + z] \\
  & = [x + (y + z)] * (x + y) + [x + (y + z)] * z \\
  & = \{[x + (y + z)] * x + [x + (y + z)] * y\} + [x * z + (y + z) * z]\\
  & = \{x + [x * y + (y + z) * y]\} + (x * z + z)\\
  & = [x + (x * y + y)] + z\\
  & = (x + y) + z
\end{align*}

so: $A = x + (y + z) = (x + y) + z$.
\end{proof}

Boundedness Laws
\begin{equation}
x + 1 = 1
\end{equation}

\begin{equation}
x * 0 = 0
\end{equation}

\begin{proof}
\begin{align*}
x + 1 & = (x + 1) * 1 \\
      & = (x + 1) * (x + x') \\
      & = x * (x + x') + 1 * (x + x') \\
      & = (x * x + x * x') + (x + x') \\
      & = (x * x') + (x + x') \\
      & = 0 + 1 \\
      & = 1
\end{align*}
\end{proof}

\end{document}
